lean/privacy/tracing/tracing.lean
@@ -1,201 +1,455 @@
 import privacy.tracing.tracing_context
 import privacy.tracing.graph
 
-def TracingContext.alice {crypto: Crypto} {m: Memory} {events: List Event}
+def TracingContext.alice {crypto: Crypto} {m: Memory} {events: List (List Event)}
     (context: TracingContext crypto m events) (coin: Coin crypto m) : UserPrivKey crypto m :=
   have h := context.h_coin_props_alice coin
-  let kalice: crypto.PrivateKeys := ⟨get_priv_key crypto events coin.esn.addralice, h.1⟩
+  let kalice: crypto.PrivateKeys := ⟨get_priv_key crypto events.flatten coin.esn.addralice, h.1⟩
   ⟨coin.esn.addralice, kalice, h.2.1⟩
 
-def TracingContext.bob {crypto: Crypto} {m: Memory} {events: List Event}
+def TracingContext.bob {crypto: Crypto} {m: Memory} {events: List (List Event)}
     (context: TracingContext crypto m events) (coin: Coin crypto m) : UserPrivKey crypto m :=
   have h := context.h_coin_props_bob coin
-  let kbob: crypto.PrivateKeys := ⟨get_priv_key crypto events coin.esn.addrbob, h.1⟩
+  let kbob: crypto.PrivateKeys := ⟨get_priv_key crypto events.flatten coin.esn.addrbob, h.1⟩
   ⟨coin.esn.addrbob, kbob, h.2.1⟩
 
+inductive OutgoingElement
+  | Note (esn: ExScannedNote)
+  | Withdrawal (evt: WithdrawalEvent)
+deriving DecidableEq
+
+def OutgoingElement.amount
+  (crypto: Crypto) (m: Memory)
+  (elm: OutgoingElement) : ℕ :=
+  match elm with
+  | OutgoingElement.Note esn => esn.amount crypto m
+  | OutgoingElement.Withdrawal evt => evt.amount
+
+def all_outgoing {crypto: Crypto} {m: Memory} {events: List (List Event)}
+    (context: TracingContext crypto m events)
+    (user: UserPrivKey crypto m) (token: ℕ) :=
+  (
+    nonopen_created_notes context.toScanOutgoingNoteContext user.addr user.k token
+    |>.map OutgoingElement.Note
+  ) ++ (
+    withdrawals_for_user_token context.toScanNoteContext events user token
+    |>.map OutgoingElement.Withdrawal
+  )
+
 def incoming_equiv_outgoing
-  {crypto: Crypto} {m: Memory} {events: List Event}
+  {crypto: Crypto} {m: Memory} {events: List (List Event)}
   (context: TracingContext crypto m events)
   (user: UserPrivKey crypto m) (token: ℕ) :=
   amounts_to_coins.equiv
     (ℓ₀ := spent_notes_ex context.toScanNoteContext user.addr user.k token)
-    (ℓ₁ := nonopen_created_notes context.toScanOutgoingNoteContext user.addr user.k token)
+    (ℓ₁ := all_outgoing context user token)
     (h_nodup₀ := by
       apply List.Nodup.filter
       apply List.Nodup.filter
       apply List.nodup_dedup
     )
     (h_nodup₁ := by
-      apply List.Nodup.filter
-      apply List.Nodup.filter
-      apply List.nodup_dedup
+      apply List.Nodup.append
+      · apply List.Nodup.map (by apply OutgoingElement.Note.inj)
+        apply List.Nodup.filter
+        apply List.Nodup.filter
+        apply List.nodup_dedup
+      · apply List.Nodup.map (by apply OutgoingElement.Withdrawal.inj)
+        apply List.Nodup.filter
+        apply withdrawals_for_user.nodup
+      · intro x h₀ h₁
+        rw [List.mem_map] at h₀ h₁
+        obtain ⟨_, _, h₀⟩ := h₀
+        obtain ⟨_, _, h₁⟩ := h₁
+        rw [←h₀] at h₁
+        contradiction
     )
     (f := λ esn ↦ esn.amount crypto m)
     (g := λ esn ↦ esn.amount crypto m)
-    (h_sum := by rw [context.h_incoming_eq_outgoing])
+    (h_sum := by
+      rw [context.h_incoming_eq_outgoing, all_outgoing, List.map_append, List.sum_append]
+      apply congrArg₂
+      · rw [List.map_map]
+        apply congrArg
+        apply List.map_congr_left
+        intro esn h_esn
+        rfl
+      · rw [List.map_map]
+        apply congrArg
+        apply List.map_congr_left
+        intro evt h_evt
+        rfl
+    )
 
-theorem TracingContext.next_coin_spent_notes_ex {crypto: Crypto} {m: Memory} {events: List Event}
+theorem TracingContext.next_coin_spent_notes_ex {crypto: Crypto} {m: Memory} {events: List (List Event)}
     (context: TracingContext crypto m events) (coin: Coin crypto m)
     (h_spent: m MemoryType.Nullifiers [crypto.hash [coin.esn.c, coin.esn.token, coin.esn.i, (context.bob coin).k]] ≠ 0) :
     let bob := context.bob coin
-    (coin.esn, coin.coin_idx) ∈ (amounts_to_coins
+    (coin.esn, coin.coin_idx) ∈ amounts_to_coins
        (spent_notes_ex context.toScanNoteContext bob.addr bob.k coin.esn.token)
-       (λ esn => esn.amount crypto m)).toFinset := by
-  simp only [List.mem_toFinset, amounts_to_coins.mem]
+       (λ esn => esn.amount crypto m) := by
+  simp only [amounts_to_coins.mem]
   refine ⟨?_, coin.h_coin_idx⟩
   simp only [spent_notes_ex, List.mem_filter, decide_eq_true_eq, and_true]
   have h := context.h_coin_props_bob coin
   refine ⟨h.2.2 h.1, h_spent⟩
 
-def TracingContext.prev_coin_helper {crypto: Crypto} {m: Memory} {events: List Event}
+theorem TracingContext.prev_coin_helper {crypto: Crypto} {m: Memory} {events: List (List Event)}
     (context: TracingContext crypto m events) (coin: Coin crypto m)
     (h_nonopen: is_open_note crypto m (coin.esn.note_id crypto) = false) :
     let alice := context.alice coin
-    (coin.esn, coin.coin_idx) ∈ (amounts_to_coins
-       (nonopen_created_notes context.toScanOutgoingNoteContext alice.addr alice.k coin.esn.token)
-       (λ esn => esn.amount crypto m)).toFinset := by
-    simp only [List.mem_toFinset, amounts_to_coins.mem]
+    (.Note coin.esn, coin.coin_idx) ∈ amounts_to_coins
+       (all_outgoing context alice coin.esn.token)
+       (λ esn => esn.amount crypto m) := by
+    simp only [amounts_to_coins.mem]
     refine ⟨?_, coin.h_coin_idx⟩
+    rw [all_outgoing, List.mem_append]
+    apply Or.inl
+    simp only [List.mem_map, OutgoingElement.Note.injEq, exists_eq_right]
     simp only [nonopen_created_notes, List.mem_filter, decide_eq_true_eq, and_true]
     have h := context.h_coin_props_alice coin
     refine ⟨h.2.2, h_nonopen⟩
 
-def TracingContext.next_coin₀ {crypto: Crypto} {m: Memory} {events: List Event}
+def TracingContext.next_coin₀ {crypto: Crypto} {m: Memory} {events: List (List Event)}
+    (context: TracingContext crypto m events) (coin: Coin crypto m) :
+    Option (OutgoingElement × ℕ) :=
+  let bob := context.bob coin
+  let incoming_outgoing := incoming_equiv_outgoing context bob coin.esn.token
+  ↑(partial_equiv incoming_outgoing ⟨coin.esn, coin.coin_idx⟩)
+
+theorem TracingContext.next_coin₀_from_some_withdrawal {crypto: Crypto} {m: Memory} {events: List (List Event)}
+    {context: TracingContext crypto m events} {coin: Coin crypto m}
+    {evt: WithdrawalEvent} {coin_idx: ℕ}
+    (h_next_coin₀: context.next_coin₀ coin = some (.Withdrawal evt, coin_idx)) :
+    coin.esn.token = evt.token ∧
+    coin.esn.addrbob = evt.addr ∧
+    coin_idx < evt.amount ∧
+    Event.Withdraw evt.user_enc evt.amount evt.token ∈ events.flatten := by
+  have h := partial_equiv_from_some h_next_coin₀
+  simp only [amounts_to_coins.mem, all_outgoing, List.mem_append, List.mem_map, reduceCtorEq,
+    and_false, exists_false, OutgoingElement.Withdrawal.injEq, exists_eq_right, false_or] at h
+  simp only [withdrawals_for_user_token, withdrawals_for_user, List.mem_filter, decide_eq_true_eq] at h
+  have ⟨_, ⟨h₀, h₁⟩, h₂⟩ := h
+  clear h
+  replace ⟨i, ⟨user_enc, amount, token⟩, h₀⟩ := mem_mapIdx' h₀
+  simp only [List.mem_flatMap] at h₀
+  replace ⟨⟨⟨events, cond⟩, h_evt, h₀⟩, h₀'⟩ := h₀
+  split at h₀
+  swap; · simp at h₀
+
+  simp only [List.mem_filterMap] at h₀
+  have ⟨_, _, h₀⟩ := h₀
+  split at h₀
+  swap; · simp at h₀
+  rename_i h_withdraw_in
+  simp only [Option.some.injEq, Prod.mk.injEq] at h₀
+  simp only [h₀] at h_withdraw_in
+
+  refine ⟨h₁.symm, ?_, h₂, ?_⟩
+  · simp [h₀']
+    rfl
+  · simp only [List.mem_flatten, h₀']
+    exact ⟨events, (List.of_mem_zip h_evt).1, h_withdraw_in⟩
+
+theorem TracingContext.next_coin₀_from_some_note {crypto: Crypto} {m: Memory} {events: List (List Event)}
+    {context: TracingContext crypto m events} {coin: Coin crypto m}
+    {esn: ExScannedNote} {coin_idx: ℕ}
+    (h_next_coin₀: context.next_coin₀ coin = some (.Note esn, coin_idx)) :
+    coin.esn.token = esn.token ∧
+    coin.esn.addrbob = esn.addralice ∧
+    coin_idx < esn.amount crypto m ∧
+    m MemoryType.Nullifiers [coin.esn.nullifier crypto (context.bob coin).k] ≠ 0 := by
+  have h := partial_equiv_from_some h_next_coin₀
+  simp only [amounts_to_coins.mem, all_outgoing, nonopen_created_notes, Bool.decide_eq_false,
+    List.filter_filter, List.mem_append, List.mem_map, List.mem_filter, Bool.and_eq_true,
+    Bool.not_eq_eq_eq_not, Bool.not_true, decide_eq_true_eq, OutgoingElement.Note.injEq,
+    exists_eq_right, reduceCtorEq, and_false, exists_false, or_false] at h
+  simp only [spent_notes_ex, ne_eq, decide_not, List.filter_filter, List.mem_filter, decide_true,
+    Bool.and_true, Bool.not_eq_eq_eq_not, Bool.not_true, decide_eq_false_iff_not] at h
+  have ⟨⟨⟨_, h_nullifier⟩, _⟩, ⟨h₀, _, h₁⟩, h₂⟩ := h
+  exact ⟨h₁.symm, (context.h_scan_outgoing_notes_for_sender _ _ _ h₀).1, h₂, h_nullifier⟩
+
+theorem TracingContext.next_coin₀_inj {crypto: Crypto} {m: Memory} {events: List (List Event)}
+    {context: TracingContext crypto m events}
+    {coin₀ coin₁: Coin crypto m}
+    {elt: OutgoingElement} {coin_idx: ℕ}
+    (h_next_coin₀: context.next_coin₀ coin₀ = some (elt, coin_idx))
+    (h_next_coin₁: context.next_coin₀ coin₁ = some (elt, coin_idx)) :
+    coin₀ = coin₁ := by
+  have ⟨h_token, h_bob⟩: coin₀.esn.token = coin₁.esn.token ∧ coin₀.esn.addrbob = coin₁.esn.addrbob := by
+    cases elt
+    case Withdrawal evt =>
+      have h₀ := context.next_coin₀_from_some_withdrawal h_next_coin₀
+      have h₁ := context.next_coin₀_from_some_withdrawal h_next_coin₁
+      simp [h₀, h₁]
+    case Note esn =>
+      have h₀ := context.next_coin₀_from_some_note h_next_coin₀
+      have h₁ := context.next_coin₀_from_some_note h_next_coin₁
+      simp [h₀, h₁]
+
+  simp only [TracingContext.next_coin₀] at h_next_coin₀ h_next_coin₁
+  apply (partial_equiv_inv _ _ _).1 at h_next_coin₀
+  apply (partial_equiv_inv _ _ _).1 at h_next_coin₁
+  have h_bob : context.bob coin₀ = context.bob coin₁ := by
+    simp [TracingContext.bob, h_bob]
+  rw [h_token, h_bob] at h_next_coin₀
+  simp only [h_next_coin₁, Option.some.injEq, Prod.mk.injEq] at h_next_coin₀
+  apply Coin.ext <;> simp [*]
+
+def TracingContext.prev_coin₀ {crypto: Crypto} {m: Memory} {events: List (List Event)}
+    (context: TracingContext crypto m events) (coin: Coin crypto m) :
+    Option (ExScannedNote × ℕ) :=
+  let alice := context.alice coin
+  let incoming_outgoing := incoming_equiv_outgoing context alice coin.esn.token
+  ↑(partial_equiv incoming_outgoing.symm ⟨.Note coin.esn, coin.coin_idx⟩)
+
+theorem TracingContext.next_coin₀_prop
+    {crypto: Crypto} {m: Memory} {events: List (List Event)}
     (context: TracingContext crypto m events) (coin: Coin crypto m)
     (h_spent: m MemoryType.Nullifiers [crypto.hash [coin.esn.c, coin.esn.token, coin.esn.i, (context.bob coin).k]] ≠ 0) :
     let bob := context.bob coin
-    { v : ExScannedNote × ℕ // v ∈ (
-      amounts_to_coins
-        (nonopen_created_notes context.toScanOutgoingNoteContext bob.addr bob.k coin.esn.token)
-        (λ esn ↦ esn.amount crypto m)
-      ).toFinset
-    } := by
+    let res := context.next_coin₀ coin
+    ∃ (elt: OutgoingElement) (coin_idx: ℕ),
+    res = some (elt, coin_idx) ∧
+    elt ∈ all_outgoing context bob coin.esn.token ∧
+    coin_idx < elt.amount crypto m := by
   intro bob
+  dsimp only [TracingContext.next_coin₀]
   let incoming_outgoing := incoming_equiv_outgoing context bob coin.esn.token
-  exact incoming_outgoing ⟨⟨coin.esn, coin.coin_idx⟩, context.next_coin_spent_notes_ex _ h_spent⟩
+  have ⟨⟨elt, coin_idx⟩, h₀, h₁⟩ := partial_equiv_prop incoming_outgoing ⟨coin.esn, coin.coin_idx⟩
+    (context.next_coin_spent_notes_ex _ h_spent)
+  use elt, coin_idx, h₀
 
-def TracingContext.prev_coin₀ {crypto: Crypto} {m: Memory} {events: List Event}
+  rw [amounts_to_coins.mem] at h₁
+  exact h₁
+
+theorem TracingContext.prev_coin₀_prop
+    {crypto: Crypto} {m: Memory} {events: List (List Event)}
     (context: TracingContext crypto m events) (coin: Coin crypto m)
     (h_nonopen: is_open_note crypto m (coin.esn.note_id crypto) = false) :
     let alice := context.alice coin
-    { v : ExScannedNote × ℕ // v ∈ (
-      amounts_to_coins
-        (spent_notes_ex context.toScanNoteContext alice.addr alice.k coin.esn.token)
-        (λ esn ↦ esn.amount crypto m)
-      ).toFinset
-    }  := by
+    let res := context.prev_coin₀ coin
+    ∃ (esn: ExScannedNote) (coin_idx: ℕ),
+    res = some (esn, coin_idx) ∧
+    esn ∈ spent_notes_ex context.toScanNoteContext alice.addr alice.k coin.esn.token  ∧
+    coin_idx < esn.amount crypto m := by
   intro alice
+  dsimp only [TracingContext.prev_coin₀]
   let incoming_outgoing := incoming_equiv_outgoing context alice coin.esn.token
-  exact incoming_outgoing.invFun ⟨⟨coin.esn, coin.coin_idx⟩, context.prev_coin_helper _ h_nonopen⟩
+  have ⟨⟨esn, coin_idx⟩, h₀, h₁⟩ := partial_equiv_prop incoming_outgoing.symm
+    ⟨.Note coin.esn, coin.coin_idx⟩
+    (context.prev_coin_helper _ h_nonopen)
+  use esn, coin_idx, h₀
+  rw [amounts_to_coins.mem] at h₁
+  exact h₁
 
 theorem TracingContext.next_prev₀
-    {crypto: Crypto} {m: Memory} {events: List Event}
-    (context: TracingContext crypto m events) (coin₀ coin₁: Coin crypto m)
-    (token: ℕ) (h_token₀: token = coin₀.esn.token)
-    (user: UserPrivKey crypto m) (h_user₀: user = context.bob coin₀)
-    (h_spent: m MemoryType.Nullifiers [crypto.hash [coin₀.esn.c, coin₀.esn.token, coin₀.esn.i, (context.bob coin₀).k]] ≠ 0)
-    (h_nonopen: is_open_note crypto m (coin₁.esn.note_id crypto) = false) :
-    context.next_coin₀ coin₀ h_spent = (coin₁.esn, coin₁.coin_idx) ↔
-    context.prev_coin₀ coin₁ h_nonopen = (coin₀.esn, coin₀.coin_idx) := by
-  set res₀ := context.next_coin₀ coin₀ h_spent with h_res₀
-  set res₁ := context.prev_coin₀ coin₁ h_nonopen with h_res₁
+    {crypto: Crypto} {m: Memory} {events: List (List Event)}
+    (context: TracingContext crypto m events) (coin₀ coin₁: Coin crypto m) :
+    context.next_coin₀ coin₀ = some (.Note coin₁.esn, coin₁.coin_idx) ↔
+    context.prev_coin₀ coin₁ = some (coin₀.esn, coin₀.coin_idx) := by
   have (a b: Prop): (a ∨ b → (a ↔ b)) → (a ↔ b) := by
     by_cases h: a; all_goals simp [h]
   apply this
-  intro h_or
 
-  have ⟨h_addr₁, h_token₁⟩ : coin₀.esn.addrbob = coin₁.esn.addralice ∧ token = coin₁.esn.token := by
+  intro h_or
+  have h_addr_token : coin₀.esn.addrbob = coin₁.esn.addralice ∧ coin₀.esn.token = coin₁.esn.token := by
+    simp only [TracingContext.next_coin₀, TracingContext.prev_coin₀] at h_or
     cases h_or
     case inl h_or =>
-      have := res₀.prop
-      rw [List.mem_toFinset, amounts_to_coins.mem] at this
-      simp only [nonopen_created_notes, List.mem_filter, decide_eq_true_eq] at this
-      have ⟨h_addralice, Kbob, h_c⟩ := context.h_scan_outgoing_notes_for_sender _ _ _ this.1.1.1
-      simp only [TracingContext.bob, h_or] at h_addralice
+      have ⟨h₀, h₁⟩ := partial_equiv_from_some h_or
+      simp [amounts_to_coins.mem] at h₀ h₁
 
-      have h_token := this.1.1.2.symm
-      simp only [h_or] at h_token
+      simp only [spent_notes_ex, List.mem_filter, decide_eq_true_eq, and_true] at h₀
+      have ⟨h_addr₀, _, _⟩ := context.h_scan_notes_for_recipient _ _ h₀.1.1
 
-      exact ⟨h_addralice, h_token₀ ▸ h_token⟩
+      simp only [all_outgoing, List.mem_append] at h₁
+      cases h₁.1
+      case inr h₁ => simp [List.mem_map] at h₁
+      rename_i h₁
+      simp only [List.mem_map, List.mem_filter, OutgoingElement.Note.injEq, exists_eq_right,
+        nonopen_created_notes, decide_eq_true_eq] at h₁
+      have ⟨h_addr₁, Kbob, _⟩ := context.h_scan_outgoing_notes_for_sender _ _ _ h₁.1.1
+
+      rw [←h_addr₀, h_addr₁, h₁.1.2]
+      trivial
     case inr h_or =>
-      have := res₁.prop
-      rw [List.mem_toFinset, amounts_to_coins.mem] at this
-      simp only [spent_notes_ex, List.mem_filter, decide_eq_true_eq] at this
-      have ⟨h_addrbob, kalice, h_c⟩ := context.h_scan_notes_for_recipient (context.alice coin₁) _ this.1.1.1
-      simp only [TracingContext.alice, h_or] at h_addrbob
+      have ⟨h₁, h₀⟩ := partial_equiv_from_some h_or
+      simp [amounts_to_coins.mem] at h₀ h₁
+      simp only [spent_notes_ex, List.mem_filter, decide_eq_true_eq] at h₀
+      have ⟨h_addr₀, _, _⟩ := context.h_scan_notes_for_recipient _ _ h₀.1.1.1
 
-      have h_token := this.1.1.2.symm
-      simp only [h_or] at h_token
+      simp only [all_outgoing, List.mem_append] at h₁
+      cases h₁.1
+      case inr h₁ => simp [List.mem_map] at h₁
+      rename_i h₁
+      simp only [List.mem_map, List.mem_filter, OutgoingElement.Note.injEq, exists_eq_right,
+        nonopen_created_notes, decide_eq_true_eq, and_true] at h₁
+      have ⟨h_addr₁, Kbob, _⟩ := context.h_scan_outgoing_notes_for_sender _ _ _ h₁.1
 
-      exact ⟨h_addrbob.symm, h_token₀ ▸ h_token.symm⟩
+      rw [←h_addr₀, h_addr₁, h₀.1.1.2]
+      trivial
 
-  replace h_user₁ : user = context.alice coin₁ := by
-    rw [h_user₀]
+  have h_user : context.bob coin₀ = context.alice coin₁ := by
     simp only [TracingContext.bob, TracingContext.alice]
-    conv => lhs; arg 1; rw [h_addr₁]
-    conv => lhs; arg 2; arg 1; rw [h_addr₁]
+    conv => enter [1, 1]; rw [h_addr_token.1]
+    conv => enter [1, 2, 1]; rw [h_addr_token.1]
 
-  let incoming_outgoing := incoming_equiv_outgoing context user token
-  have h_res₀' : res₀.1 = (incoming_outgoing ⟨⟨coin₀.esn, coin₀.coin_idx⟩, h_token₀ ▸ h_user₀ ▸ context.next_coin_spent_notes_ex _ h_spent⟩).1 := by
-    cases h_token₀
-    cases h_user₀
-    rfl
-  have h_res₁' : res₁.1 = (incoming_outgoing.symm ⟨⟨coin₁.esn, coin₁.coin_idx⟩, h_token₁ ▸ h_user₁ ▸ context.prev_coin_helper _ h_nonopen⟩).1 := by
-    cases h_token₁
-    cases h_user₁
-    rfl
+  simp only [TracingContext.next_coin₀, TracingContext.prev_coin₀]
+  rw [h_user, h_addr_token.2]
+  apply partial_equiv_inv
 
-  rw [h_res₀']
-  have (S: Type) (p q: S → Prop) (e: Equiv { s // p s } { s // q s}) (x y: S) (h_x: p x) (h_y: q y):
-      ↑(e ⟨x, h_x⟩) = y ↔ ↑(e.symm ⟨y, h_y⟩) = x := by
-    have : e ⟨x, h_x⟩ = ⟨y, h_y⟩ ↔ ↑(e ⟨x, h_x⟩) = y := by apply Subtype.ext_iff
-    rw [←this]
+-------------------------------------
 
-    have : e.symm ⟨y, h_y⟩ = ⟨x, h_x⟩ ↔ ↑(e.symm ⟨y, h_y⟩) = x := by apply Subtype.ext_iff
-    rw [←this]
+def TracingContext.next_coin₁ {crypto: Crypto} {m: Memory} {events: List (List Event)}
+    (context: TracingContext crypto m events) (coin: Coin crypto m) :
+    Option (ExScannedNote × ℕ) :=
+  let res := context.next_coin₀ coin
+  match res with
+  | some (OutgoingElement.Note esn, coin_idx) => some ⟨esn, coin_idx⟩
+  | _ => none
 
-    rw [e.apply_eq_iff_eq_symm_apply]
-    constructor
-    all_goals intro h; rw [h]
-
-  rw [this, h_res₁']
-
-def TracingContext.next_coin₁ {crypto: Crypto} {m: Memory} {events: List Event}
-    (context: TracingContext crypto m events) (coin: Coin crypto m)
-    (h_spent: m MemoryType.Nullifiers [crypto.hash [coin.esn.c, coin.esn.token, coin.esn.i, (context.bob coin).k]] ≠ 0) :
-    Coin crypto m := by
-  let ⟨⟨esn, coin_idx⟩, h_next⟩ := context.next_coin₀ coin h_spent
-
-  simp only [List.mem_toFinset, amounts_to_coins.mem, nonopen_created_notes, List.mem_filter, decide_eq_true_eq] at h_next
-  refine ⟨esn, coin_idx, h_next.2, ?_⟩
-  have ⟨h_addralice, Kbob, h_c⟩ := context.h_scan_outgoing_notes_for_sender _ _ _ h_next.1.1.1
-  use (context.bob coin).k, Kbob, h_c
-
-def TracingContext.prev_coin₁ {crypto: Crypto} {m: Memory} {events: List Event}
-    (context: TracingContext crypto m events) (coin: Coin crypto m)
-    (h_nonopen: is_open_note crypto m (coin.esn.note_id crypto) = false) :
-    Coin crypto m := by
-  let ⟨⟨esn, coin_idx⟩, h_prev⟩ := context.prev_coin₀ coin h_nonopen
-
-  simp only [List.mem_toFinset, amounts_to_coins.mem, spent_notes_ex, List.mem_filter, decide_eq_true_eq] at h_prev
-  refine ⟨esn, coin_idx, h_prev.2, ?_⟩
-  have ⟨h_addrbob, kalice, h_c⟩ := context.h_scan_notes_for_recipient (context.alice coin) _ h_prev.1.1.1
-  use kalice, crypto.priv_to_pub (context.alice coin).k, h_c
+def TracingContext.prev_coin₁ {crypto: Crypto} {m: Memory} {events: List (List Event)}
+    (context: TracingContext crypto m events) (coin: Coin crypto m) :
+    Option (ExScannedNote × ℕ) :=
+  context.prev_coin₀ coin
 
 theorem TracingContext.next_prev₁
-    {crypto: Crypto} {m: Memory} {events: List Event}
+    {crypto: Crypto} {m: Memory} {events: List (List Event)}
+    (context: TracingContext crypto m events) (coin₀ coin₁: Coin crypto m) :
+    context.next_coin₁ coin₀ = some ⟨coin₁.esn, coin₁.coin_idx⟩ ↔
+    context.prev_coin₁ coin₁ = some ⟨coin₀.esn, coin₀.coin_idx⟩ := by
+  simp only [TracingContext.next_coin₁, TracingContext.prev_coin₁]
+  constructor
+  · split
+    · rename_i res esn coin_idx h
+      intro h'
+      simp only [Option.some.injEq, Prod.mk.injEq] at h'
+      rw [h'.1, h'.2] at h
+      exact (context.next_prev₀ _ _).1 h
+    · intro h
+      contradiction
+  · split
+    · rename_i res esn coin_idx h
+      intro h'
+      rw [(context.next_prev₀ _ _).2 h'] at h
+      simp only [Option.some.injEq, Prod.mk.injEq, OutgoingElement.Note.injEq] at h
+      simp [h]
+    · rename_i res h
+      intro h'
+      exfalso
+      have := (context.next_prev₀ _ _).2 h'
+      exact h coin₁.esn coin₁.coin_idx this
+
+-------------------------------------
+
+def TracingContext.next_coin₂ {crypto: Crypto} {m: Memory} {events: List (List Event)}
+    (context: TracingContext crypto m events) (coin: Coin crypto m)
+    (h_spent: m MemoryType.Nullifiers [crypto.hash [coin.esn.c, coin.esn.token, coin.esn.i, (context.bob coin).k]] ≠ 0) :
+    Option (Coin crypto m) :=
+  match h: context.next_coin₁ coin with
+  | some ⟨esn, coin_idx⟩ => by
+    refine some ⟨esn, coin_idx, ?_, ?_⟩
+    all_goals
+      have prop := context.next_coin₀_prop coin h_spent
+      simp only [TracingContext.next_coin₁] at h
+      cases h' : context.next_coin₀ coin
+      case none => simp [h'] at h
+      rename_i val
+      have h_val : val = (val.1, val.2) := by rfl
+      cases h'': val.1
+      case Withdrawal esn' =>
+        rw [h', h_val, h''] at h
+        simp at h
+      rename_i esn'
+      rw [h', h_val, h'', Option.some.injEq, Prod.mk.injEq] at h
+      have ⟨elt, coin_idx', prop₀, prop₁, prop₂⟩ := prop
+      clear prop
+      rw [h', Option.some.injEq, Prod.mk.injEq, h.2, h''] at prop₀
+
+    · simp only [←prop₀, OutgoingElement.amount, h] at prop₂
+      exact prop₂
+    · rw [all_outgoing, List.mem_append] at prop₁
+      cases prop₁
+      case inl prop₁ =>
+        simp only [←prop₀, h, List.mem_map] at prop₁
+        simp only [OutgoingElement.Note.injEq, exists_eq_right,
+          nonopen_created_notes, List.mem_filter, decide_eq_true_eq] at prop₁
+        have ⟨h_addralice, Kbob, h_c⟩ := context.h_scan_outgoing_notes_for_sender _ _ _ prop₁.1.1
+        exact ⟨(context.bob coin).k, Kbob, h_c⟩
+      case inr prop₁ =>
+        simp [←prop₀] at prop₁
+  | none => none
+
+def TracingContext.prev_coin₂ {crypto: Crypto} {m: Memory} {events: List (List Event)}
+    (context: TracingContext crypto m events) (coin: Coin crypto m)
+    (h_nonopen: is_open_note crypto m (coin.esn.note_id crypto) = false) :
+    Option (Coin crypto m) :=
+  match h: context.prev_coin₁ coin with
+  | some ⟨esn, coin_idx⟩ => by
+    refine some ⟨esn, coin_idx, ?_, ?_⟩
+    all_goals
+      have prop := context.prev_coin₀_prop coin h_nonopen
+      simp only [TracingContext.prev_coin₁] at h
+      cases h' : context.prev_coin₀ coin
+      case none => simp [h'] at h
+      rename_i val
+      rw [h', Option.some.injEq, Prod.mk.injEq] at h
+      have ⟨esn', coin_idx', prop₀, prop₁, prop₂⟩ := prop
+      clear prop
+      rw [h', Option.some.injEq, Prod.mk.injEq, h.2] at prop₀
+
+    · simp only [←prop₀, h] at prop₂
+      exact prop₂
+    · simp only [←prop₀, h] at prop₁
+      simp only [spent_notes_ex, List.mem_filter, decide_eq_true_eq] at prop₁
+      have ⟨h_addrbob, kalice, h_c⟩ := context.h_scan_notes_for_recipient _ _ prop₁.1.1
+      exact ⟨_, _, h_c⟩
+  | none => none
+
+theorem TracingContext.next_prev₂
+    {crypto: Crypto} {m: Memory} {events: List (List Event)}
     (context: TracingContext crypto m events) (coin₀ coin₁: Coin crypto m)
     (h_spent: m MemoryType.Nullifiers [crypto.hash [coin₀.esn.c, coin₀.esn.token, coin₀.esn.i, (context.bob coin₀).k]] ≠ 0)
     (h_nonopen: is_open_note crypto m (coin₁.esn.note_id crypto) = false) :
-    context.next_coin₁ coin₀ h_spent = coin₁ ↔
-    context.prev_coin₁ coin₁ h_nonopen = coin₀ := by
-  simp only [TracingContext.next_coin₁, TracingContext.prev_coin₁]
-  simp only [Coin.ext_iff]
-  have := context.next_prev₀ coin₀ coin₁ _ (by rfl) _ (by rfl) h_spent h_nonopen
-  simp only [Prod.ext_iff] at this
-  exact this
+    context.next_coin₂ coin₀ h_spent = some coin₁ ↔
+    context.prev_coin₂ coin₁ h_nonopen = some coin₀ := by
+  simp only [TracingContext.next_coin₂, TracingContext.prev_coin₂]
+  split
+  · rename_i esn coin_idx h_next
+    split
+    · rename_i esn' coin_idx' h_prev
+      simp only [Option.some.injEq, Coin.ext_iff]
+      constructor
+      · intro h
+        simp [h] at h_next
+        replace h_next := (context.next_prev₁ _ _).1 h_next
+        rw [h_next, Option.some.injEq, Prod.mk.injEq] at h_prev
+        simp [h_prev]
+      · intro h
+        simp [h] at h_prev
+        replace h_prev := (context.next_prev₁ _ _).2 h_prev
+        rw [h_prev, Option.some.injEq, Prod.mk.injEq] at h_next
+        simp [h_next]
+    · rename_i h_none
+      simp only [Option.some.injEq, reduceCtorEq, iff_false, Coin.ext_iff]
+      by_contra h
+      simp [h] at h_next
+      replace h_next := (context.next_prev₁ _ _).1 h_next
+      simp [h_next] at h_none
+  · rename_i h_none
+    split
+    · simp only [Option.some.injEq, Coin.ext_iff, reduceCtorEq, false_iff]
+      rename_i esn' coin_idx' h_prev
+      by_contra h
+      simp [h] at h_prev
+      replace h_prev := (context.next_prev₁ _ _).2 h_prev
+      simp [h_prev] at h_none
+    · simp
 
-def TracingContext.next_coin {crypto: Crypto} {m: Memory} {events: List Event}
+-------------------------------------
+
+def TracingContext.next_coin {crypto: Crypto} {m: Memory} {events: List (List Event)}
   (context: TracingContext crypto m events)
   (coin: Coin crypto m) : Option (Coin crypto m) := by
   let bob := context.bob coin
@@ -204,10 +458,10 @@ def TracingContext.next_coin {crypto: Crypto} {m: Memory} {events: List Event}
   by_cases h_is_spent: m MemoryType.Nullifiers [crypto.hash [coin.esn.c, coin.esn.token, coin.esn.i, bob.k]] ≠ 0
   case neg => exact none
 
-  exact some (context.next_coin₁ coin h_is_spent)
+  exact context.next_coin₂ coin h_is_spent
 
 def TracingContext.prev_coin
-    {crypto: Crypto} {m: Memory} {events: List Event}
+    {crypto: Crypto} {m: Memory} {events: List (List Event)}
     (context: TracingContext crypto m events)
     (coin: Coin crypto m) :
     Option (Coin crypto m) := by
@@ -217,63 +471,122 @@ def TracingContext.prev_coin
   by_cases h_nonopen: is_open_note crypto m (coin.esn.note_id crypto)
   case pos => exact none
 
-  exact some (context.prev_coin₁ coin (by simp only [h_nonopen]))
-
-theorem TracingContext.next_coin_none
-    {crypto: Crypto} {m: Memory} {events: List Event}
-    (context: TracingContext crypto m events)
-    (coin: Coin crypto m) :
-    context.next_coin coin = none ↔
-    m MemoryType.Nullifiers [crypto.hash [coin.esn.c, coin.esn.token, coin.esn.i, (context.bob coin).k]] = 0 := by
-  simp only [TracingContext.next_coin]
-  split_ifs <;> simp [*]; omega
-
-theorem TracingContext.prev_coin_none
-    {crypto: Crypto} {m: Memory} {events: List Event}
-    (context: TracingContext crypto m events)
-    (coin: Coin crypto m) :
-    context.prev_coin coin = none ↔
-    is_open_note crypto m (coin.esn.note_id crypto) := by
-  simp only [TracingContext.prev_coin]
-  split_ifs <;> simp [*]
+  exact context.prev_coin₂ coin (by simp only [h_nonopen])
 
 theorem TracingContext.next_prev
-    {crypto: Crypto} {m: Memory} {events: List Event}
+    {crypto: Crypto} {m: Memory} {events: List (List Event)}
     (context: TracingContext crypto m events)
     (coin₀ coin₁: Coin crypto m) :
     context.next_coin coin₀ = some coin₁ ↔
     context.prev_coin coin₁ = some coin₀ := by
   simp only [TracingContext.next_coin, TracingContext.prev_coin]
-  simp only [ne_eq, dite_not, Option.dite_none_left_eq_some, Option.some.injEq, Bool.not_eq_true]
+  simp only [ne_eq, dite_not, Option.dite_none_left_eq_some, Bool.not_eq_true]
   constructor
   · intro ⟨h_spent, h⟩
     have h_nonopen : is_open_note crypto m (ScannedNote.note_id crypto coin₁.esn.toScannedNote) = false := by
-      rw [←h]
-      simp only [TracingContext.next_coin₁]
-      set res := context.next_coin₀ coin₀ h_spent
-      have := res.prop
-      rw [List.mem_toFinset, amounts_to_coins.mem] at this
-      simp only [nonopen_created_notes, List.mem_filter, decide_eq_true_eq] at this
-      exact this.1.2
-    have := context.next_prev₁ coin₀ coin₁ h_spent h_nonopen
+      have ⟨elt, _, prop₀, prop₁, _⟩ := context.next_coin₀_prop coin₀ h_spent
+
+      simp only [TracingContext.next_coin₂, TracingContext.next_coin₁] at h
+      split at h
+      swap
+      · contradiction
+      rename_i esn _ h'
+
+      split at h'
+      swap
+      · contradiction
+      rename_i res esn' _ h''
+
+      simp only [Option.some.injEq, Coin.ext_iff] at h
+      rw [prop₀, Option.some.injEq, Prod.mk.injEq] at h''
+      simp only [Option.some.injEq, Prod.mk.injEq] at h'
+      simp only [all_outgoing, List.mem_append] at prop₁
+      cases prop₁
+      swap
+      · rename_i h_elt_in
+        simp [List.mem_map, h''] at h_elt_in
+
+      rename_i h_elt_in
+      simp only [h'', List.mem_map, OutgoingElement.Note.injEq,
+        exists_eq_right] at h_elt_in
+      simp only [nonopen_created_notes, List.mem_filter, decide_eq_true_eq, h'.1] at h_elt_in
+
+      rw [←h.1]
+      exact h_elt_in.2
+
+    have := context.next_prev₂ coin₀ coin₁ h_spent h_nonopen
     use h_nonopen, this.1 h
   · intro ⟨h_nonopen, h⟩
     have h_nullifier : m MemoryType.Nullifiers [crypto.hash [coin₀.esn.c, coin₀.esn.token, coin₀.esn.i, ↑(context.bob coin₀).k]] ≠ 0 := by
-      rw [←h]
-      simp only [TracingContext.prev_coin₁]
-      set res := context.prev_coin₀ coin₁ h_nonopen
-      have := res.prop
-      rw [List.mem_toFinset, amounts_to_coins.mem] at this
-      simp only [spent_notes_ex, List.mem_filter, decide_eq_true_eq] at this
+      have ⟨esn, _, prop₀, prop₁, _⟩ := context.prev_coin₀_prop coin₁ h_nonopen
+      simp only [TracingContext.prev_coin₂, TracingContext.prev_coin₁] at h
+      split at h
+
+      swap
+      · contradiction
+      rename_i esn' _ h'
+
+      simp only [Option.some.injEq, Coin.ext_iff] at h
+      rw [prop₀, Option.some.injEq, Prod.mk.injEq] at h'
+
+      simp only [spent_notes_ex, List.mem_filter, decide_eq_true_eq] at prop₁
       simp only [TracingContext.bob]
-      have h_addr := (context.h_scan_notes_for_recipient (context.alice coin₁) _ this.1.1.1).1
-      rw [←h_addr]
-      exact this.1.2
-    have := context.next_prev₁ coin₀ coin₁ h_nullifier h_nonopen
+
+      have h_addr := (context.h_scan_notes_for_recipient (context.alice coin₁) _ prop₁.1.1).1
+      simp only [←h.1, ←h'.1, ←h_addr]
+
+      exact prop₁.2
+    have := context.next_prev₂ coin₀ coin₁ h_nullifier h_nonopen
     use h_nullifier, this.2 h
 
+theorem TracingContext.next_coin_none
+    {crypto: Crypto} {m: Memory} {events: List (List Event)}
+    (context: TracingContext crypto m events)
+    (coin: Coin crypto m) :
+    context.next_coin coin = none ↔
+    m MemoryType.Nullifiers [crypto.hash [coin.esn.c, coin.esn.token, coin.esn.i, (context.bob coin).k]] = 0 ∨
+    ∃ (evt: WithdrawalEvent) (coin_idx: ℕ), context.next_coin₀ coin = some (.Withdrawal evt, coin_idx)
+     := by
+  simp only [TracingContext.next_coin, TracingContext.next_coin₂]
+  by_cases h_spent: m MemoryType.Nullifiers [crypto.hash [coin.esn.c, coin.esn.token, coin.esn.i, (context.bob coin).k]] = 0
+  case pos => simp [h_spent]
+  case neg =>
+    simp only [ne_eq, h_spent, not_false_eq_true, ↓reduceDIte, false_or]
+    have ⟨elt, coin_idx, prop₀, prop₁, prop₂⟩ := context.next_coin₀_prop coin h_spent
+    simp only [prop₀, Option.some.injEq, Prod.mk.injEq, exists_and_left, ↓existsAndEq, and_true]
+
+    split
+    · simp only [reduceCtorEq, false_iff]
+      by_contra h_next_coin₀
+      obtain ⟨evt, h_next_coin₀⟩ := h_next_coin₀
+      rename_i h_next_coin₁
+      simp [TracingContext.next_coin₁, prop₀, h_next_coin₀] at h_next_coin₁
+    · simp only [true_iff]
+      cases elt
+      case Withdrawal evt => use evt
+      case Note esn =>
+        rename_i h_next_coin₁
+        simp [TracingContext.next_coin₁, prop₀] at h_next_coin₁
+
+theorem TracingContext.prev_coin_none
+    {crypto: Crypto} {m: Memory} {events: List (List Event)}
+    (context: TracingContext crypto m events)
+    (coin: Coin crypto m) :
+    context.prev_coin coin = none ↔
+    is_open_note crypto m (coin.esn.note_id crypto) := by
+  simp only [TracingContext.prev_coin, TracingContext.prev_coin₂, TracingContext.prev_coin₁]
+  split
+  · simp [*]
+  · split
+    · simp [*]
+    · rename_i h
+      have ⟨esn, coin_idx, prop₀, prop₁, prop₂⟩ := context.prev_coin₀_prop coin (by simp only [*])
+      simp [h] at prop₀
+
+-------------------------------------
+
 def TracingContext.tracing_graph
-    {crypto: Crypto} {m: Memory} {events: List Event}
+    {crypto: Crypto} {m: Memory} {events: List (List Event)}
     (context: TracingContext crypto m events) :
     Graph (Coin crypto m) := {
   next := context.next_coin
