lean/privacy/tracing/withdrawals.lean
@@ -1,0 +1,66 @@
+import privacy.actions
+import privacy.amounts
+import privacy.compliance.all_notes
+import privacy.notes.used_notes
+import privacy.registration.discoverable
+import privacy.tracing.utils
+import privacy.transactions.transactions
+import privacy.transactions.withdrawals
+
+theorem withdrawals_for_user_token_sum
+    {crypto: Crypto} (stxs: SuccessfulTransactions crypto)
+    (user: UserPrivKey crypto stxs.rm.m) (token: ℕ) :
+    (
+      withdrawals_for_user_token (.from stxs.rm) stxs.events user token
+      |>.map (λ evt ↦ evt.amount)
+      |>.sum
+    ) = (
+      stxs.txs
+      |>.filter (λ tx ↦ tx.owner = user.addr)
+      |>.map (λ tx ↦ tx.sum_withdraw_amounts token)
+      |>.sum
+    ) := by
+  unfold withdrawals_for_user_token
+  rw [withdrawals_for_user.eq]
+  rw [mapIdx_filter_map
+    (h_p := by intros; simp)
+    (h_q := by intros; simp)
+  ]
+
+  simp only [List.flatMap_reverse, List.filter_reverse, List.map_reverse, List.sum_reverse]
+  simp only [List.filter_flatMap, List.map_flatMap]
+  conv => rhs; rw [←List.filterMap_eq_filter, List.map_filterMap]
+  rw [List.filterMap_eq_flatMap_toList]
+  unfold List.flatMap
+  rw [List.sum_flatten, List.sum_flatten]
+  apply congrArg
+  simp only [List.map_map]
+  apply List.map_congr_left
+  intro tx h_tx
+
+  by_cases h_owner: tx.owner = user.addr
+  case neg =>
+    simp [h_owner, Option.guard]
+  case pos =>
+    simp [h_owner, Transaction₀.sum_amounts]
+    apply congrArg
+    simp only [List.filter_filterMap, List.map_filterMap]
+    apply List.filterMap_congr
+    intro action h_action
+
+    simp [ActionFunc.withdraw, filter_Withdraw]
+    cases action
+    case Withdraw inp =>
+      simp only [Option.map_some, Option.filter_some]
+      split
+      case isTrue h_token =>
+        simp only [decide_eq_true_eq] at h_token
+        simp only [h_token, Option.map_some, decide_eq_true_eq, Option.map_if,
+          Option.some_eq_ite_none_right, Option.some.injEq]
+        exact ⟨h_token, by rfl⟩
+      case isFalse h_token =>
+        simp only [decide_eq_true_eq] at h_token
+        simp
+        exact h_token
+
+    all_goals simp
